src/Utils/Maps.v
@@ -1,0 +1,79 @@
+Require Import Lists.List.
+Import ListNotations.
+From coqutil Require Import Map.Interface Map.Properties.
+
+From Utils Require Import Base Lists NamedList Eqb.
+
+(* TODO: move has_key here from Sep *)
+Section __.
+  Context (A B : Type)
+    (mp : map.map A B)
+    (m_ok : map.ok mp)
+    (A_Eqb : Eqb A)
+    (A_Eqb_ok : Eqb_ok A_Eqb).
+
+  Lemma map_keys_in (m : mp) k
+    : In k (map.keys m) -> exists v, map.get m k = Some v.
+  Proof.
+    unfold map.keys.
+    rewrite Properties.map.fold_to_tuples_fold.
+    rewrite fold_right_map_fst.
+    intro.
+    
+    apply pair_fst_in_exists in H.
+    break.
+    exists x.
+    eapply map.tuples_spec.
+    auto.
+  Qed.
+  
+  Lemma map_keys_in' (m : mp) k
+    : In k (map.keys m) <-> if map.get m k then True else False.
+  Proof.
+    case_match; intuition eauto.
+    {
+      eapply Properties.map.in_keys; eauto.
+    }
+    {
+      eapply map_keys_in in H;
+        basic_goal_prep.
+      congruence.
+    }
+  Qed.
+  
+  Lemma map_split_incl2 (a x x0 : mp)
+    : map.split a x x0 ->
+      incl (map.keys a) (map.keys x ++ map.keys x0).
+  Proof.
+    intros Hsplit i Hin.
+    autorewrite with utils.
+    rewrite !map_keys_in' in *.
+    eapply Properties.map.get_split with (k:=i) in Hsplit; eauto.
+    intuition subst.
+    {
+      rewrite H1, <- H0.
+      case_match; eauto.
+    }
+    {
+      rewrite H1, <- H0.
+      case_match; eauto.
+    }
+  Qed.
+
+  
+  Lemma map_keys_empty : map.keys (map:=mp) map.empty = [].
+  Proof.
+    unfold map.keys.
+    basic_utils_crush.
+    apply map.fold_empty.
+  Qed.
+  Hint Rewrite map_keys_empty : utils.
+
+End __.
+
+
+Arguments map_keys_in {A B}%type_scope {mp m_ok A_Eqb A_Eqb_ok} m k _.
+Arguments map_keys_in' {A B}%type_scope {mp m_ok A_Eqb A_Eqb_ok} m k.
+
+
+#[export] Hint Rewrite map_keys_empty : utils.
